Cleanup; add dependent.lean

src/circuits/circuit_encoding.lean
@@ -4,54 +4,6 @@ import polytime.lemmas
 open tencodable tree
 open_locale tree complexity_class
 
-section
-variables {α : Type*} {β : α → Type*}
-
-lemma multiset.nodupkeys_iff {s : multiset (sigma β)} :
-  s.nodupkeys ↔ s.keys.nodup := quotient.induction_on s $ λ l, iff.rfl
-
-lemma finmap.keysnodup (f : finmap β) : f.entries.keys.nodup := multiset.nodupkeys_iff.mp f.nodupkeys
-
-def finmap.of_fun [fintype α] (f : Π x, β x) :
-  finmap β :=
-{ entries := finset.univ.val.map (λ x : α, ⟨x, f x⟩),
-  nodupkeys := by simpa [multiset.nodupkeys_iff, multiset.keys] using finset.univ.nodup }
-
-lemma finmap.mem_lookup_iff [decidable_eq α] {f : finmap β} {x : α} (y : β x) :
-   f.lookup x = some y ↔ (⟨x, y⟩ : sigma β) ∈ f.entries :=
-finmap.induction_on f (λ a, alist.mem_lookup_iff) 
-
-@[simp] lemma finmap.of_fun_lookup [fintype α] [decidable_eq α] {f : Π x, β x} (x : α) :
-  (finmap.of_fun f).lookup x = some (f x) :=
-by { rw finmap.mem_lookup_iff, exact multiset.mem_map_of_mem _ (finset.mem_univ_val x), }
-
-def finmap.comap {α β γ : Type*} (m : @finmap α (λ _, β)) (f : α ↪ γ) : @finmap γ (λ _, β) :=
-{ entries := m.entries.map (λ x, ⟨f x.1, x.2⟩),
-  nodupkeys := multiset.nodupkeys_iff.mpr (by simpa [multiset.keys] using m.keysnodup.map f.2) }
-
-def finmap.disj_union {α β γ : Type*} (m₁ : @finmap α (λ _, γ)) (m₂ : @finmap β (λ _, γ)) : @finmap (α ⊕ β) (λ _, γ) :=
-{ entries := m₁.entries.map (λ x, ⟨sum.inl x.1, x.2⟩) + m₂.entries.map (λ x, ⟨sum.inr x.1, x.2⟩),
-  nodupkeys := begin
-    rw [multiset.nodupkeys_iff, multiset.keys, multiset.map_add, multiset.nodup_add],
-    refine ⟨_, _, _⟩,
-    { simpa [multiset.keys] using m₁.keysnodup.map sum.inl_injective, },
-    { simpa [multiset.keys] using m₂.keysnodup.map sum.inr_injective, },
-    { simp [multiset.disjoint], }
-  end }
-
-@[simp] lemma finmap.disj_union_lookup_left {α β γ : Type*} [decidable_eq α] [decidable_eq β] (m₁ : @finmap α (λ _, γ)) (m₂ : @finmap β (λ _, γ)) (x : α) :
-  (m₁.disj_union m₂).lookup (sum.inl x) = m₁.lookup x :=
-by { ext y, simp [finmap.mem_lookup_iff, finmap.disj_union], }
-
-@[simp] lemma finmap.disj_union_lookup_right {α β γ : Type*} [decidable_eq α] [decidable_eq β] (m₁ : @finmap α (λ _, γ)) (m₂ : @finmap β (λ _, γ)) (x : β) :
-  (m₁.disj_union m₂).lookup (sum.inr x) = m₂.lookup x :=
-by { ext y, simp [finmap.mem_lookup_iff, finmap.disj_union], }
-
-def finmap.map {γ : α → Type*} (m : finmap β) (f : ∀ x, β x → γ x) : finmap γ :=
-{ entries := m.entries.map (λ x, ⟨x.1, f x.1 x.2⟩),
-  nodupkeys := by simpa [multiset.nodupkeys_iff, multiset.keys] using m.keysnodup }
-
-end
 
 variables {α β U V W X : Type}
 
